lambda2Gmu/InfrastructureSubst.v
@@ -65,14 +65,6 @@ Proof.
   rewrite* subst_tt_fresh. simpl. case_var*.
 Qed.
 
-(* possibly move to Defs *)
-Fixpoint subst_tt_many (Xs : list var) (Us : list typ) (T : typ) :=
-  match (Xs, Us) with
-  (* | ((List.cons X Xt), (List.cons U Ut)) => subst_tt X U (subst_tt_many Xt Ut T) *)
-  | ((List.cons X Xt), (List.cons U Ut)) => subst_tt_many Xt Ut (subst_tt X U T)
-  | _ => T
-  end.
-
 Lemma subst_commutes_with_unrelated_opens : forall Xs T V Y,
     (forall X, List.In X Xs -> X <> Y) ->
     type V ->
@@ -485,13 +477,6 @@ Proof.
       * apply* IHvalue.
 Qed.
 
-
-Fixpoint subst_tb_many (As : list var) (Us : list typ) (b : bind) : bind :=
-  match (As, Us) with
-  | (List.cons Ah At, List.cons Uh Ut) => subst_tb_many At Ut (subst_tb Ah Uh b)
-  | _ => b
-  end.
-
 (* Lemma adding_free_is_ok : forall A E F, *)
 (*     ok (E & F) -> *)
 (*     A # E -> *)
@@ -724,4 +709,56 @@ Lemma subst_te_many_commutes_open : forall As Ts e x,
     rewrite IHAts; auto with listin.
     f_equal.
     apply subst_te_open_ee_var.
+Qed.
+
+Lemma subst_tb_id_on_fresh : forall E Z P,
+    Z \notin fv_env E ->
+    map (subst_tb Z P) E = E.
+  induction E using env_ind; introv FE.
+  - rewrite map_empty. trivial.
+  - rewrite map_push.
+    destruct v.
+    rewrite fv_env_extend in FE.
+    f_equal.
+    + apply* IHE.
+    + cbn.
+      f_equal. f_equal.
+      apply subst_tt_fresh. auto.
+Qed.
+
+Lemma subst_tt_many_id_on_fresh : forall T As Ps,
+    (forall A, List.In A As -> A \notin fv_typ T) ->
+    subst_tt_many As Ps T = T.
+  induction As; destruct Ps; intros; try solve [cbn in *; congruence].
+  cbn.
+  rewrite subst_tt_fresh.
+  - apply IHAs; auto with listin.
+  - auto with listin.
+Qed.
+
+Lemma subst_tb_many_id_on_fresh_env : forall E As Ps,
+    length As = length Ps ->
+    (forall A, List.In A As -> A \notin fv_env E) ->
+    map (subst_tb_many As Ps) E = E.
+  intros.
+  rewrite map_def.
+  rewrite <- LibList_map.
+  symmetry.
+  rewrite <- map_id; auto.
+  intros vb xin.
+  destruct vb. cbn.
+  f_equal; auto.
+  unfold subst_tb_many. destruct b.
+  rewrite subst_tt_many_id_on_fresh; auto.
+  intros.
+  induction E as [| B E].
+  - contradiction.
+  - lets HA: H0 H1.
+    cbn in HA. fold (fv_env E) in HA.
+    lets [? | ?]: List.in_inv xin; subst; cbn in HA; auto.
+    apply IHE; auto.
+    intros A' Ain.
+    lets HA': H0 Ain.
+    destruct B; destruct b; cbn in HA'. fold (fv_env E) in HA'.
+    auto.
 Qed.
